library/init/data/sigma/basic.lean
@@ -14,10 +14,16 @@ universes u v
 lemma ex_of_psig {α : Type u} {p : α → Prop} : (Σ' x, p x) → ∃ x, p x
 | ⟨x, hx⟩ := ⟨x, hx⟩
 
-namespace sigma
-  variables {α : Type u} {β : α → Type v}
+section
+variables {α : Type u} {β : α → Type v}
 
-  protected lemma eq : ∀ {p₁ p₂ : Σ a : α, β a} (h₁ : p₁.1 = p₂.1), (eq.rec_on h₁ p₁.2 : β p₂.1) = p₂.2 → p₁ = p₂
-  | ⟨a, b⟩ ⟨.a, .b⟩ rfl rfl := rfl
+protected lemma sigma.eq : ∀ {p₁ p₂ : Σ a : α, β a} (h₁ : p₁.1 = p₂.1), (eq.rec_on h₁ p₁.2 : β p₂.1) = p₂.2 → p₁ = p₂
+| ⟨a, b⟩ ⟨.a, .b⟩ rfl rfl := rfl
+end
 
-end sigma
+section
+variables {α : Sort u} {β : α → Sort v}
+
+protected lemma psigma.eq : ∀ {p₁ p₂ : psigma β} (h₁ : p₁.1 = p₂.1), (eq.rec_on h₁ p₁.2 : β p₂.1) = p₂.2 → p₁ = p₂
+| ⟨a, b⟩ ⟨.a, .b⟩ rfl rfl := rfl
+end
