tests/lean/run/funext_issue.lean
@@ -1,0 +1,4 @@
+universes u
+
+example (α : Type u) (p : Prop) (a b : α) (h : p → a = b) : (λ x : p, a) = (λ x : p, b) :=
+funext h
